infrastructural update, inst spec except initialisers state interp update and pure items

theories/iris/iris_host.v
@@ -698,7 +698,88 @@ Definition import_resources_wasm_typecheck (v_imps: list module_export) (t_imps:
   | MED_global (Mk_globalidx i) => (∃ g gt, N.of_nat i ↦[wg] g ∗ ⌜ wgs !! (N.of_nat i) = Some g /\ t = ET_glob gt /\ global_agree g gt ⌝)
   end.
 
+(*
+(* An alternate definition that splits the above into the four different components from the start. *)
+Definition import_resources_wasm_typecheck_split (v_imps: list module_export) (t_imps: list extern_t) (wfs: gmap N function_closure) (wts: gmap N tableinst) (wms: gmap N memory) (wgs: gmap N global): iProp Σ :=
+  import_resources_wasm_domcheck v_imps wfs wts wms wgs ∗
+  ([∗ list] i ↦ v; t ∈ (ext_func_addrs (fmap modexp_desc v_imps)); (ext_t_funcs t_imps), ∃ cl, N.of_nat v ↦[wf] cl ∗ ⌜ wfs !! (N.of_nat v) = Some cl /\ t = (cl_type cl)⌝) ∗
+  ([∗ list] i ↦ v; t ∈ (ext_tab_addrs (fmap modexp_desc v_imps)); (ext_t_tabs t_imps), ∃ tab, N.of_nat v ↦[wtblock] tab ∗ ⌜ wts !! (N.of_nat v) = Some tab /\ tab_typing tab t ⌝) ∗
+  ([∗ list] i ↦ v; t ∈ (ext_mem_addrs (fmap modexp_desc v_imps)); (ext_t_mems t_imps), ∃ mem, N.of_nat v ↦[wmblock] mem ∗ ⌜ wms !! (N.of_nat v) = Some mem /\ mem_typing mem t ⌝) ∗
+  ([∗ list] i ↦ v; t ∈ (ext_glob_addrs (fmap modexp_desc v_imps)); (ext_t_globs t_imps), ∃ g, N.of_nat v ↦[wg] g ∗ ⌜ wgs !! (N.of_nat v) = Some g /\ global_agree g t ⌝).
 
+(* Note that the original definition applies the alt, but not the other way round. *)
+Lemma import_resources_wasm_equivalent_aux (v_imps: list module_export) (t_imps: list extern_t) (wfs: gmap N function_closure) (wts: gmap N tableinst) (wms: gmap N memory) (wgs: gmap N global):
+  (*import_resources_wasm_domcheck v_imps wfs wts wms wgs*) ⊢
+  (([∗ list] i ↦ v; t ∈ v_imps; t_imps,
+  match v.(modexp_desc) with
+  | MED_func (Mk_funcidx i) => ((∃ cl, N.of_nat i ↦[wf] cl ∗ ⌜ wfs !! (N.of_nat i) = Some cl /\ t = ET_func (cl_type cl) ⌝)%I)
+  | MED_table (Mk_tableidx i) => (∃ tab tt, N.of_nat i ↦[wtblock] tab ∗ ⌜ wts !! (N.of_nat i) = Some tab /\ t = ET_tab tt /\ tab_typing tab tt ⌝)
+  | MED_mem (Mk_memidx i) => (∃ mem mt, N.of_nat i ↦[wmblock] mem ∗ ⌜ wms !! (N.of_nat i) = Some mem /\ t = ET_mem mt /\ mem_typing mem mt ⌝) 
+  | MED_global (Mk_globalidx i) => (∃ g gt, N.of_nat i ↦[wg] g ∗ ⌜ wgs !! (N.of_nat i) = Some g /\ t = ET_glob gt /\ global_agree g gt ⌝) end) ↔
+  (([∗ list] i ↦ v; t ∈ (ext_func_addrs (fmap modexp_desc v_imps)); (ext_t_funcs t_imps), ∃ cl, N.of_nat v ↦[wf] cl ∗ ⌜ wfs !! (N.of_nat v) = Some cl /\ t = (cl_type cl)⌝) ∗
+  ([∗ list] i ↦ v; t ∈ (ext_tab_addrs (fmap modexp_desc v_imps)); (ext_t_tabs t_imps), ∃ tab, N.of_nat v ↦[wtblock] tab ∗ ⌜ wts !! (N.of_nat v) = Some tab /\ tab_typing tab t ⌝) ∗
+  ([∗ list] i ↦ v; t ∈ (ext_mem_addrs (fmap modexp_desc v_imps)); (ext_t_mems t_imps), ∃ mem, N.of_nat v ↦[wmblock] mem ∗ ⌜ wms !! (N.of_nat v) = Some mem /\ mem_typing mem t ⌝) ∗
+  ([∗ list] i ↦ v; t ∈ (ext_glob_addrs (fmap modexp_desc v_imps)); (ext_t_globs t_imps), ∃ g, N.of_nat v ↦[wg] g ∗ ⌜ wgs !! (N.of_nat v) = Some g /\ global_agree g t ⌝)))%I.
+Proof.
+  move: wgs wms wts wfs t_imps.
+  iInduction v_imps as [ | v] "IH"; iIntros (wgs wms wts wfs t_imps) => /=; destruct t_imps => //=.
+  - iSplit; first by iIntros "?" => //=.
+    destruct e; by iIntros "(?&?&?&?)".
+  - iSplit; first by iIntros "?".
+    destruct v, modexp_desc => /=; by iIntros "(?&?&?&?)".
+  - iSplit.
+    + destruct v, modexp_desc; iIntros "(Hhead & Htail)" => /=.
+      * destruct f.
+        iDestruct "Hhead" as (cl) "(Hhead & %Hhead)".
+        destruct Hhead as [Hlookup ->].
+        iSimpl.
+        unfold ext_tab_addrs, ext_mem_addrs, ext_glob_addrs.
+        simpl.
+        iDestruct ("IH" with "Htail") as "(Hf & Ht & Hm & Hg)".
+        iFrame.
+        iExists cl; by iFrame.
+      * destruct t.
+        iDestruct "Hhead" as (tab tt) "(Hhead & %Hhead)".
+        destruct Hhead as [Hlookup [-> Htt]].
+        iSimpl.
+        unfold ext_func_addrs, ext_mem_addrs, ext_glob_addrs.
+        simpl.
+        iDestruct ("IH" with "Htail") as "(Hf & Ht & Hm & Hg)".
+        iFrame.
+        iExists tab; by iFrame.
+      * destruct m.
+        iDestruct "Hhead" as (mem mt) "(Hhead & %Hhead)".
+        destruct Hhead as [Hlookup [-> Hmt]].
+        iSimpl.
+        unfold ext_func_addrs, ext_tab_addrs, ext_glob_addrs.
+        simpl.
+        iDestruct ("IH" with "Htail") as "(Hf & Ht & Hm & Hg)".
+        iFrame.
+        iExists mem; by iFrame.
+      * destruct g.
+        iDestruct "Hhead" as (glob gt) "(Hhead & %Hhead)".
+        destruct Hhead as [Hlookup [-> Hgt]].
+        iSimpl.
+        unfold ext_func_addrs, ext_tab_addrs, ext_mem_addrs.
+        simpl.
+        iDestruct ("IH" with "Htail") as "(Hf & Ht & Hm & Hg)".
+        iFrame.
+        iExists glob; by iFrame.
+   (* + destruct v, modexp_desc; iIntros "(Hf & Ht & Hm & Hg)" => /=.
+      * destruct f.
+        unfold ext_func_addrs => /=.
+        unfold oapp.
+        iDestruct ("IH" with "Hf Ht Hm Hg") as "Hcons".
+        iDestruct (big_sepL2_length with "Hf") as "%Hlength".
+        simpl in Hlength.
+        destruct e => //=.
+        admit.
+        iDestruct (big_sepL2_length with "Hf") as "%Hlength2".
+        iDestruct "Hf" as "(Hhead & Htail)".*)
+        admit.
+Admitted.
+        
+*)
 Definition exp_default := MED_func (Mk_funcidx 0).
 
 (* The resources for module exports. This is a bit more complicated since it is allowed to export the imported elements,
@@ -723,6 +804,46 @@ Definition module_export_resources_host (v_imps: list module_export) (hs_exps: l
                                                    end
                                                    ).
 
+
+Lemma ext_tabs_lookup_exist (modexps: list module_export_desc) n tn:
+  (ext_tabs modexps) !! n = Some tn ->
+  exists k, modexps !! k = Some (MED_table tn).
+Proof.
+  move: n tn.
+  induction modexps; move => n tn Hexttablookup => //=.
+  simpl in Hexttablookup.
+  destruct a => //. 
+  2: { simpl in *.
+       destruct n; simpl in *; first by inversion Hexttablookup; subst; exists 0.
+       apply IHmodexps in Hexttablookup.
+       destruct Hexttablookup as [k ?].
+       by exists (S k).
+  }
+  all: simpl in *. 
+  all: apply IHmodexps in Hexttablookup.
+  all: destruct Hexttablookup as [k ?].
+  all: by exists (S k).
+Qed.
+
+Lemma ext_mems_lookup_exist (modexps: list module_export_desc) n mn:
+  (ext_mems modexps) !! n = Some mn ->
+  exists k, modexps !! k = Some (MED_mem mn).
+Proof.
+  move: n mn.
+  induction modexps; move => n mn Hextmemlookup => //=.
+  simpl in Hextmemlookup.
+  destruct a => //. 
+  3: { simpl in *.
+       destruct n; simpl in *; first try by inversion Hextmemlookup; subst; exists 0.
+       apply IHmodexps in Hextmemlookup.
+       destruct Hextmemlookup as [k ?].
+       by exists (S k).
+  }
+  all: simpl in *. 
+  all: apply IHmodexps in Hextmemlookup.
+  all: destruct Hextmemlookup as [k ?].
+  all: by exists (S k).
+Qed.
 
 Lemma import_resources_host_lookup hs_imps v_imps vis:
   ⊢ ghost_map_auth visGName 1 vis -∗
@@ -810,7 +931,181 @@ Proof.
     exists g, gt.
     by repeat split => //.
 Qed.
-    
+
+
+Lemma import_resources_wts_subset v_imps t_imps wfs wts wms wgs (ws: store_record):
+  ⊢ gen_heap_interp (gmap_of_table (s_tables ws)) -∗
+    gen_heap_interp (gmap_of_list (fmap tab_size (s_tables ws))) -∗
+    gen_heap_interp (gmap_of_list (fmap table_max_opt (s_tables ws))) -∗
+    import_resources_wasm_typecheck v_imps t_imps wfs wts wms wgs -∗
+    ⌜ length v_imps = length t_imps ⌝ -∗
+    ⌜ wts ⊆ gmap_of_list (s_tables ws) ⌝.
+Proof.
+  iIntros "Hwt Hwtsize Hwtlimit (%Himpwasmdom & Himpwasm) %Himplen".
+  rewrite map_subseteq_spec.
+  iIntros (i x Hwtslookup).
+  destruct Himpwasmdom as [_ [Hwtdom _]].
+  assert (i ∈ dom (gset N) wts) as Hidom.
+  { by apply elem_of_dom. }
+  rewrite -> Hwtdom in Hidom.
+  rewrite -> elem_of_list_to_set in Hidom.
+
+  unfold ext_tab_addrs, compose in Hidom.
+  rewrite -> elem_of_list_fmap in Hidom.
+  destruct Hidom as [? [-> Hidom]].
+  rewrite -> elem_of_list_fmap in Hidom.
+  destruct Hidom as [t [-> Hidom]].
+  destruct t.
+  rewrite -> elem_of_list_lookup in Hidom.
+  destruct Hidom as [k Hdom].
+  apply ext_tabs_lookup_exist in Hdom.
+  destruct Hdom as [k' Hdom].
+  rewrite list_lookup_fmap in Hdom.
+  destruct (v_imps !! k') eqn:Hvimpslookup => //.
+  simpl in Hdom.
+
+  inversion Hdom; clear Hdom.
+
+  assert (exists t, t_imps !! k' = Some t) as Htimpslookup.
+  { apply lookup_lt_Some in Hvimpslookup.
+    rewrite Himplen in Hvimpslookup.
+    destruct (t_imps !! k') eqn:Htimpslookup; try by eexists.
+    apply lookup_ge_None in Htimpslookup.
+    by lias.
+  }
+
+  destruct Htimpslookup as [t Htimpslookup].
+  
+  iDestruct (big_sepL2_lookup with "Himpwasm") as "Hvimp" => //.
+  rewrite H0.
+  iDestruct "Hvimp" as (tab tt) "(Htab & %Hwts)".
+  destruct Hwts as [Hwtslookup' [-> Htt]].
+  rewrite Hwtslookup in Hwtslookup'.
+  inversion Hwtslookup'; subst; clear Hwtslookup'.
+
+  iDestruct (tab_block_lookup with "Hwt Hwtsize Hwtlimit Htab") as "%Hwtblock".
+
+  rewrite gmap_of_list_lookup.
+
+  by rewrite Hwtblock.
+Qed.
+
+Definition mem_equiv (m1 m2: memory): Prop :=
+  m1.(mem_max_opt) = m2.(mem_max_opt) /\
+  m1.(mem_data).(ml_data) = m2.(mem_data).(ml_data).
+
+Definition map_related {K: Type} {M: Type -> Type} {H0: forall A: Type, Lookup K A (M A)} {A: Type} (r: relation A) (m1 m2: M A) :=
+  forall (i: K) (x: A), m1 !! i = Some x -> exists y, m2 !! i = Some y /\ r x y.
+
+Lemma import_resources_wms_subset v_imps t_imps wfs wts wms wgs (ws: store_record):
+  ⊢ gen_heap_interp (gmap_of_memory (s_mems ws)) -∗
+    gen_heap_interp (gmap_of_list (fmap mem_length (s_mems ws))) -∗
+    gen_heap_interp (gmap_of_list (fmap mem_max_opt (s_mems ws))) -∗
+    import_resources_wasm_typecheck v_imps t_imps wfs wts wms wgs -∗
+    ⌜ length v_imps = length t_imps ⌝ -∗
+    ⌜ map_related mem_equiv wms (gmap_of_list (s_mems ws)) ⌝.
+Proof.
+  iIntros "Hwm Hwmlength Hwmlimit (%Himpwasmdom & Himpwasm) %Himplen".
+  unfold map_related.
+  iIntros (i x Hwmslookup).
+  destruct Himpwasmdom as [_ [_ [Hwmdom _]]].
+  assert (i ∈ dom (gset N) wms) as Hidom.
+  { by apply elem_of_dom. }
+  rewrite -> Hwmdom in Hidom.
+  rewrite -> elem_of_list_to_set in Hidom.
+
+  unfold ext_mem_addrs, compose in Hidom.
+  rewrite -> elem_of_list_fmap in Hidom.
+  destruct Hidom as [? [-> Hidom]].
+  rewrite -> elem_of_list_fmap in Hidom.
+  destruct Hidom as [memid [-> Hidom]].
+  destruct memid.
+  rewrite -> elem_of_list_lookup in Hidom.
+  destruct Hidom as [k Hdom].
+  apply ext_mems_lookup_exist in Hdom.
+  destruct Hdom as [k' Hdom].
+  rewrite list_lookup_fmap in Hdom.
+  destruct (v_imps !! k') eqn:Hvimpslookup => //.
+  simpl in Hdom.
+
+  inversion Hdom; clear Hdom.
+
+  assert (exists t, t_imps !! k' = Some t) as Htimpslookup.
+  { apply lookup_lt_Some in Hvimpslookup.
+    rewrite Himplen in Hvimpslookup.
+    destruct (t_imps !! k') eqn:Htimpslookup; try by eexists.
+    apply lookup_ge_None in Htimpslookup.
+    by lias.
+  }
+
+  destruct Htimpslookup as [t Htimpslookup].
+  
+  iDestruct (big_sepL2_lookup with "Himpwasm") as "Hvimp" => //.
+  rewrite H0.
+  iDestruct "Hvimp" as (mem mt) "(Hmem & %Hwms)".
+  destruct Hwms as [Hwmslookup' [-> Hmt]].
+  rewrite Hwmslookup in Hwmslookup'.
+  inversion Hwmslookup'; subst; clear Hwmslookup'.
+
+  iDestruct (mem_block_lookup with "Hwm Hwmlength Hwmlimit Hmem") as "%Hwmblock".
+
+  destruct Hwmblock as [mem' [Hwmlookup [Hmdata Hmmax]]].
+
+  rewrite gmap_of_list_lookup.
+
+  rewrite Hwmlookup.
+  by iExists mem'.
+Qed.
+
+Lemma module_elem_bound_check_gmap_extend wts1 wts2 imp_descs m:
+  module_elem_bound_check_gmap wts1 imp_descs m ->
+  wts1 ⊆ wts2 ->
+  module_elem_bound_check_gmap wts2 imp_descs m.
+Proof.
+  move => Hbc Hsubset.
+  unfold module_elem_bound_check_gmap in *.
+  rewrite -> List.Forall_forall in Hbc.
+  apply List.Forall_forall.
+  move => x Hin.
+  specialize (Hbc x Hin).
+  destruct x.
+  destruct modelem_table.
+  destruct (assert_const1_i32 modelem_offset) eqn:Hoffseti32 => //.
+  destruct (ext_tabs imp_descs !! n) eqn:Himpslookup => //.
+  destruct t.
+  destruct (wts1 !! N.of_nat n0) eqn:Hwts1lookup => //.
+  replace (wts2 !! N.of_nat n0) with (Some t) => //.
+  by erewrite lookup_weaken => //.
+Qed.
+
+Lemma module_data_bound_check_gmap_extend wms1 wms2 imp_descs m:
+  module_data_bound_check_gmap wms1 imp_descs m ->
+  map_related mem_equiv wms1 wms2 ->
+  module_data_bound_check_gmap wms2 imp_descs m.
+Proof.
+  move => Hbc Hrelate.
+  unfold module_data_bound_check_gmap in *.
+  rewrite -> List.Forall_forall in Hbc.
+  apply List.Forall_forall.
+  move => x Hin.
+  specialize (Hbc x Hin).
+  destruct x.
+  destruct moddata_data.
+  destruct (assert_const1_i32 moddata_offset) eqn:Hoffseti32 => //.
+  destruct (ext_mems imp_descs !! n) eqn:Himpslookup => //.
+  destruct m0.
+  destruct (wms1 !! N.of_nat n0) eqn:Hwms1lookup => //.
+  unfold map_related in Hrelate.
+  specialize (Hrelate _ _ Hwms1lookup).
+  destruct Hrelate as [mem [Hwms2lookup Hmequiv]].
+  rewrite Hwms2lookup.
+  unfold mem_equiv in Hmequiv.
+  destruct Hmequiv as [_ Hmdata].
+  replace (mem_length mem) with (mem_length m0) => //.
+  unfold mem_length, memory_list.mem_length.
+  by rewrite Hmdata.
+Qed.
+
 Definition gen_index offset len : list nat :=
   imap (fun i x => i+offset+x) (repeat 0 len).
 
@@ -856,13 +1151,21 @@ Proof.
     f_equal.
     by apply IHl1.
 Qed.
-  
+
+Definition gen_func_instance mf inst : function_closure :=
+  let ft := nth match modfunc_type mf with
+                | Mk_typeidx n => n
+                end (inst_types inst) (Tf [] []) in
+  FC_func_native inst ft (modfunc_locals mf) (modfunc_body mf).
+                
+
 (* This is an actual interesting proof, technically *)
 (* TODO: see if it's possible to refactor the 4 proofs into one *)
 Lemma alloc_func_gen_index modfuncs ws inst ws' l:
   alloc_funcs host_function ws modfuncs inst = (ws', l) ->
   map (fun x => match x with | Mk_funcidx i => i end) l = gen_index (length (s_funcs ws)) (length modfuncs) /\
-  length ws'.(s_funcs) = length ws.(s_funcs) + length modfuncs /\
+  ws'.(s_funcs) = ws.(s_funcs) ++ fmap (fun mf => gen_func_instance mf inst) modfuncs /\
+ (* length ws'.(s_funcs) = length ws.(s_funcs) + length modfuncs /\*)
   ws.(s_tables) = ws'.(s_tables) /\
   ws.(s_mems) = ws'.(s_mems) /\
   ws.(s_globals) = ws'.(s_globals).
@@ -873,8 +1176,9 @@ Proof.
   generalize dependent ws.
   induction modfuncs using List.rev_ind; move => ws ws' l Hallocfuncs.
   - inversion Hallocfuncs; subst; clear Hallocfuncs.
-    split => //.
-    by lias.
+    simpl.
+    repeat split => //.
+    by rewrite app_nil_r.
   - rewrite fold_left_app in Hallocfuncs.
     remember (fold_left _ modfuncs (ws,[])) as fold_res.
     simpl in Hallocfuncs.
@@ -884,18 +1188,22 @@ Proof.
     inversion Hallocfuncs; subst; clear Hallocfuncs.
     rewrite map_app app_length /=.
     rewrite gen_index_extend.
-    repeat split; try by eapply IHmodfuncs; rewrite Heqfold_res.
-    + by repeat (f_equal; first by eapply IHmodfuncs; rewrite Heqfold_res).
-    + rewrite app_length => /=.
-      rewrite PeanoNat.Nat.add_assoc.
+    specialize (IHmodfuncs ws ws0 (rev l0)).
+    destruct IHmodfuncs as [? [? [? [? ?]]]]; first by rewrite Heqfold_res.
+    repeat split => //; try by eapply IHmodfuncs; rewrite Heqfold_res.
+    + rewrite H.
+      rewrite H0.
+      by rewrite app_length map_length.
+    + rewrite H0.
+      rewrite - app_assoc.
       f_equal.
-      by eapply IHmodfuncs; rewrite Heqfold_res.
+      by rewrite -> list_fmap_app.
 Qed.
 
 Lemma alloc_tab_gen_index modtabtypes ws ws' l:
   alloc_tabs host_function ws modtabtypes = (ws', l) ->
   map (fun x => match x with | Mk_tableidx i => i end) l = gen_index (length (s_tables ws)) (length modtabtypes) /\
-  ws'.(s_tables) = ws.(s_tables) ++ map (fun '{| tt_limits := {| lim_min := min; lim_max := maxo |} |} => {| table_data := repeat None (ssrnat.nat_of_bin min); table_max_opt := maxo |}) modtabtypes /\
+  ws'.(s_tables) = ws.(s_tables) ++ fmap (fun '{| tt_limits := {| lim_min := min; lim_max := maxo |} |} => {| table_data := repeat None (ssrnat.nat_of_bin min); table_max_opt := maxo |}) modtabtypes /\
   ws.(s_funcs) = ws'.(s_funcs) /\
   ws.(s_mems) = ws'.(s_mems) /\
   ws.(s_globals) = ws'.(s_globals).
@@ -931,13 +1239,13 @@ Proof.
     + rewrite H0.
       rewrite - app_assoc.
       f_equal.
-      by rewrite map_app => /=.
+      by rewrite -> list_fmap_app => /=.
 Qed.
 
 Lemma alloc_mem_gen_index modmemtypes ws ws' l:
   alloc_mems host_function ws modmemtypes = (ws', l) ->
   map (fun x => match x with | Mk_memidx i => i end) l = gen_index (length (s_mems ws)) (length modmemtypes) /\
-  ws'.(s_mems) = ws.(s_mems) ++ map (fun '{| lim_min := min; lim_max := maxo |} => {| mem_data := mem_make #00%byte (page_size * min)%N; mem_max_opt := maxo |}) modmemtypes /\
+  ws'.(s_mems) = ws.(s_mems) ++ fmap (fun '{| lim_min := min; lim_max := maxo |} => {| mem_data := mem_make #00%byte (page_size * min)%N; mem_max_opt := maxo |}) modmemtypes /\
   ws.(s_funcs) = ws'.(s_funcs) /\
   ws.(s_tables) = ws'.(s_tables) /\
   ws.(s_globals) = ws'.(s_globals).
@@ -967,18 +1275,19 @@ Proof.
     repeat split => //.
     + rewrite H.
       rewrite H0.
-      by rewrite app_length map_length.
+      by rewrite app_length fmap_length.
     + rewrite H0.
       rewrite - app_assoc.
       f_equal.
-      by rewrite map_app => /=.
+      by rewrite -> list_fmap_app => /=.
 Qed.
 
 Lemma alloc_glob_gen_index modglobs ws g_inits ws' l:
   length g_inits = length modglobs ->
   alloc_globs host_function ws modglobs g_inits = (ws', l) ->
   map (fun x => match x with | Mk_globalidx i => i end) l = gen_index (length (s_globals ws)) (length modglobs) /\
-  length ws'.(s_globals) = length ws.(s_globals) + length modglobs /\
+  ws'.(s_globals) = ws.(s_globals) ++ fmap (fun '({| modglob_type := gt; modglob_init := ge |}, v) => {| g_mut := gt.(tg_mut); g_val := v |} ) (combine modglobs g_inits) /\
+ (* length ws'.(s_globals) = length ws.(s_globals) + length modglobs /\*)
   ws.(s_funcs) = ws'.(s_funcs) /\
   ws.(s_tables) = ws'.(s_tables) /\
   ws.(s_mems) = ws'.(s_mems).
@@ -990,8 +1299,8 @@ Proof.
   generalize dependent g_inits.
   induction modglobs using List.rev_ind; move => g_inits ws ws' l Hlen Halloc.
   - inversion Halloc; subst; clear Halloc.
-    split => //.
-    by lias.
+    repeat split => //=.
+    by rewrite app_nil_r.
   - destruct g_inits using List.rev_ind; first by destruct modglobs => /=.
     repeat rewrite app_length in Hlen; simpl in Hlen.
     repeat rewrite - cat_app in Halloc.
@@ -1010,12 +1319,24 @@ Proof.
     inversion Halloc; subst; clear Halloc.
     rewrite map_app app_length /=.
     rewrite gen_index_extend.
-    repeat split; try by eapply IHmodglobs with (g_inits := g_inits) (ws' := ws0); [ lias | rewrite Heqfold_res ].
-    + by repeat (f_equal; first eapply IHmodglobs with (g_inits := g_inits) (ws' := ws0); (try by lias); (try by rewrite Heqfold_res)).
-    + rewrite app_length => /=.
-      rewrite PeanoNat.Nat.add_assoc.
+    specialize (IHmodglobs g_inits ws ws0 (rev l0)).
+    destruct IHmodglobs as [? [? [? [? ?]]]] => //.
+    + by lias.
+    + by rewrite Heqfold_res.
+    repeat split => //.
+    + rewrite H.
+      rewrite H0.
+      rewrite app_length fmap_length combine_length.
+      repeat f_equal.
+      by lias.
+    + rewrite H0.
+      rewrite - app_assoc.
       f_equal.
-      by eapply IHmodglobs with (g_inits := g_inits) (ws' := ws0); [ lias | rewrite Heqfold_res ].
+      rewrite combine_app => /=.
+      rewrite -> list_fmap_app => /=.
+      repeat f_equal.
+      destruct x => //.
+      by lias.
 Qed.
 
 
@@ -1385,46 +1706,6 @@ Proof.
     by lias.
 Qed.
 
-Lemma ext_tabs_lookup_exist (modexps: list module_export_desc) n tn:
-  (ext_tabs modexps) !! n = Some tn ->
-  exists k, modexps !! k = Some (MED_table tn).
-Proof.
-  move: n tn.
-  induction modexps; move => n tn Hexttablookup => //=.
-  simpl in Hexttablookup.
-  destruct a => //. 
-  2: { simpl in *.
-       destruct n; simpl in *; first by inversion Hexttablookup; subst; exists 0.
-       apply IHmodexps in Hexttablookup.
-       destruct Hexttablookup as [k ?].
-       by exists (S k).
-  }
-  all: simpl in *. 
-  all: apply IHmodexps in Hexttablookup.
-  all: destruct Hexttablookup as [k ?].
-  all: by exists (S k).
-Qed.
-
-Lemma ext_mems_lookup_exist (modexps: list module_export_desc) n mn:
-  (ext_mems modexps) !! n = Some mn ->
-  exists k, modexps !! k = Some (MED_mem mn).
-Proof.
-  move: n mn.
-  induction modexps; move => n mn Hextmemlookup => //=.
-  simpl in Hextmemlookup.
-  destruct a => //. 
-  3: { simpl in *.
-       destruct n; simpl in *; first try by inversion Hextmemlookup; subst; exists 0.
-       apply IHmodexps in Hextmemlookup.
-       destruct Hextmemlookup as [k ?].
-       by exists (S k).
-  }
-  all: simpl in *. 
-  all: apply IHmodexps in Hextmemlookup.
-  all: destruct Hextmemlookup as [k ?].
-  all: by exists (S k).
-Qed.
-
 Lemma fold_left_preserve {A B: Type} (P: A -> Prop) (f: A -> B -> A) (l: list B) (acc: A) :
   P acc ->
   (forall (x:A) (act: B), P x -> P (f x act)) ->
@@ -1451,11 +1732,222 @@ Proof.
     rewrite insert_length//. }
 Qed.
 
+Lemma insert_exports_none_len vis iexps exps:
+  insert_exports vis iexps exps = None ->
+  length iexps <> length exps.
+Proof.
+  move: iexps exps vis.
+  induction iexps; intros => //.
+  destruct exps => //=.
+  move => Hlen.
+  inversion Hlen; clear Hlen.
+  simpl in H.
+  destruct (insert_exports vis iexps exps) eqn:H0 => //.
+  by eapply IHiexps in H1 => //.
+Qed.
+
+
+
+
+Section instantiation_det.
+
+Lemma module_typing_det m it1 et1 it2 et2:
+  module_typing m it1 et1 ->
+  module_typing m it2 et2 ->
+  (it1, et1) = (it2, et2).
+Proof.
+  move => Hmt1 Hmt2.
+  unfold module_typing in Hmt1, Hmt2.
+  destruct m.
+  destruct Hmt1 as [fts1 [gts1 [Hmft1 [Hmtt1 [Hmmt1 [Hmgt1 [Hmet1 [Hmdt1 [Hmst1 [Hmimt1 Hmext1]]]]]]]]]].
+  destruct Hmt2 as [fts2 [gts2 [Hmft2 [Hmtt2 [Hmmt2 [Hmgt2 [Hmet2 [Hmdt2 [Hmst2 [Hmimt2 Hmext2]]]]]]]]]].
+Admitted.
+  
+Lemma instantiate_det s m vimps res res':
+  instantiate s m vimps res ->
+  instantiate s m vimps res' ->
+  res = res'.
+Proof.
+  move => Hinst1 Hinst2.
+  destruct res as [[[s1 inst1] exp1] start1].
+  destruct res' as [[[s2 inst2] exp2] start2].
+  unfold instantiate, instantiation.instantiate in *.
+  destruct Hinst1 as [t_imps1 [t_exps1 [hs1 [ws1 [g_inits1 [e_offs1 [d_offs1 [Hmodtype1 [Hexttype1 [Hallocmodule1 [Hinstglob1 [Hinstelem1 [Hinstdata1 [Hcbelem1 [Hcbdata1 [Hcstart1 Hws1]]]]]]]]]]]]]]]].
+  destruct Hinst2 as [t_imps2 [t_exps2 [hs2 [ws2 [g_inits2 [e_offs2 [d_offs2 [Hmodtype2 [Hexttype2 [Hallocmodule2 [Hinstglob2 [Hinstelem2 [Hinstdata2 [Hcbelem2 [Hcbdata2 [Hcstart2 Hws2]]]]]]]]]]]]]]]].
+Admitted.
+
+End instantiation_det.
+
+
 Ltac forward H Hname :=
   lazymatch type of H with
   | ?Hx -> _ => let Hp := fresh "Hp" in
               assert Hx as Hp; last specialize (H Hp) as Hname end.
 
+  
+Lemma alloc_func_state_update funcs funcs' nf:
+  funcs' = funcs ++ nf ->
+  gen_heap_interp (gmap_of_list funcs) -∗ |==> 
+  ((gen_heap_interp (gmap_of_list funcs')) ∗
+   ([∗ list] i ↦ v ∈ nf, N.of_nat (length funcs + i) ↦[wf] v)).
+Proof.
+  move => Hfuncs; subst.
+  iIntros "Hf".
+  specialize (gmap_of_list_append_big funcs nf) as Hgmap.
+  destruct Hgmap as [Hgunion Hgdisj].
+  rewrite Hgunion.
+  iDestruct (gen_heap_alloc_big with "Hf") as "Hf" => //.
+  iMod "Hf".
+  iModIntro.
+  iDestruct "Hf" as "(Hf & Hfmaps & Hftoken)".
+  rewrite map_union_comm => //.
+  iFrame.
+  rewrite big_opM_map_to_list.
+  rewrite map_to_list_to_map; last first.
+  (* TODO: refactor this proof *)
+  { apply NoDup_fmap_fst.
+    { move => x0 y3 z4 Hin1 Hin2.
+      apply elem_of_lookup_imap in Hin1 as [i1 [z1 [Heq3 Hl3]]].
+      apply elem_of_lookup_imap in Hin2 as [i2 [z2 [Heq4 Hl4]]].
+      inversion Heq3; subst; clear Heq3.
+      inversion Heq4; subst; clear Heq4.
+      replace i2 with i1 in Hl4; last by lias.
+      rewrite Hl3 in Hl4.
+      by inversion Hl4.
+    }
+    {
+      apply nodup_imap_inj1.
+      move => n1 n2 t1 t2 H2.
+      inversion H2; subst; clear H2.
+      by lias.
+    }
+  }
+  clear Hgunion Hgdisj.
+  iClear "Hftoken".
+  iInduction nf as [ | f'] "IH" using List.rev_ind => //=.
+  rewrite imap_app.
+  repeat rewrite big_sepL_app.
+  iDestruct "Hfmaps" as "(Hfm1 & Hfm2)".
+  iSplitL "Hfm1"; first by iApply "IH".
+  simpl.
+  by iFrame.
+Qed.
+
+Lemma alloc_tab_state_update tabs tabs' nt:
+  tabs' = tabs ++ nt ->
+  gen_heap_interp (gmap_of_table tabs) -∗
+  gen_heap_interp (gmap_of_list (fmap tab_size tabs)) -∗
+  gen_heap_interp (gmap_of_list (fmap table_max_opt tabs)) -∗ |==> 
+  ((gen_heap_interp (gmap_of_table tabs')) ∗
+   (gen_heap_interp (gmap_of_list (fmap tab_size tabs'))) ∗
+   (gen_heap_interp (gmap_of_list (fmap table_max_opt tabs'))) ∗
+   ([∗ list] i ↦ v ∈ nt, N.of_nat (length tabs + i) ↦[wtblock] v)).
+Proof.
+  move => Htabs; subst.
+  iIntros "Ht Htsize Htlim".
+  unfold gmap_of_table.
+  specialize (gmap_of_list_2d_append_big (fmap table_to_list tabs) (fmap table_to_list nt)) as Hgmap.
+  destruct Hgmap as [Hgunion Hgdisj].
+  rewrite <- fmap_app in Hgunion.
+  rewrite Hgunion.
+  iDestruct (gen_heap_alloc_big with "Ht") as "Ht" => //.
+  iMod "Ht".
+  iModIntro.
+  iDestruct "Ht" as "(Ht & Htmaps & Httoken)".
+  rewrite map_union_comm => //.
+  iFrame.
+  rewrite big_opM_map_to_list.
+  rewrite map_to_list_to_map; last first.
+  { apply NoDup_fmap_fst.
+    { move => [a0 b0] y3 z4 Hin1 Hin2.
+      apply elem_of_list_fmap in Hin1 as [[[i1 j1] x1] [Heq1 Hl1]].
+      apply elem_of_list_fmap in Hin2 as [[[i2 j2] x2] [Heq2 Hl2]].
+      inversion Heq1; subst; clear Heq1.
+      inversion Heq2; subst; clear Heq2.
+      apply flatten_2d_list_lookup in Hl1.
+      apply flatten_2d_list_lookup in Hl2.
+      assert (i1 = i2); first by lias.
+      subst. clear H0.
+      rewrite Hl1 in Hl2.
+      by inversion Hl2.
+    }
+    {
+      apply NoDup_fmap; last by apply flatten_2d_list_nodup.
+      unfold Inj.
+      move => n1 n2 H2.
+      destruct n1 as [[i1 j1] x1].
+      destruct n2 as [[i2 j2] x2].
+      inversion H2; subst; clear H2.
+      repeat f_equal.
+      by lias.
+    }
+  }
+  clear Hgunion Hgdisj.
+  iClear "Httoken".
+  iInduction nt as [ | t'] "IH" using List.rev_ind => //=.
+  repeat rewrite big_sepL_app.
+Admitted.
+  
+Lemma alloc_mem_state_update mems mems' nm:
+  mems' = mems ++ nm ->
+  gen_heap_interp (gmap_of_memory mems) -∗
+  gen_heap_interp (gmap_of_list (fmap mem_length mems)) -∗
+  gen_heap_interp (gmap_of_list (fmap mem_max_opt mems)) -∗ |==> 
+  ((gen_heap_interp (gmap_of_memory mems')) ∗
+   (gen_heap_interp (gmap_of_list (fmap mem_length mems'))) ∗
+   (gen_heap_interp (gmap_of_list (fmap mem_max_opt mems'))) ∗
+   ([∗ list] i ↦ v ∈ nm, N.of_nat (length mems + i) ↦[wmblock] v)).
+Proof.
+Admitted.
+  
+Lemma alloc_glob_state_update globs globs' ng:
+  globs' = globs ++ ng ->
+  gen_heap_interp (gmap_of_list globs) -∗ |==> 
+  ((gen_heap_interp (gmap_of_list globs')) ∗
+  ([∗ list] i ↦ v ∈ ng, N.of_nat (length globs + i) ↦[wg] v)).
+Proof.
+  move => Hglobs; subst.
+  iIntros "Hg".
+  specialize (gmap_of_list_append_big globs ng) as Hgmap.
+  destruct Hgmap as [Hgunion Hgdisj].
+  rewrite Hgunion.
+  iDestruct (gen_heap_alloc_big with "Hg") as "Hg" => //.
+  iMod "Hg".
+  iModIntro.
+  iDestruct "Hg" as "(Hg & Hgmaps & Hgtoken)".
+  rewrite map_union_comm => //.
+  iFrame.
+  rewrite big_opM_map_to_list.
+  rewrite map_to_list_to_map; last first.
+  (* TODO: refactor this proof *)
+  { apply NoDup_fmap_fst.
+    { move => x0 y3 z4 Hin1 Hin2.
+      apply elem_of_lookup_imap in Hin1 as [i1 [z1 [Heq3 Hl3]]].
+      apply elem_of_lookup_imap in Hin2 as [i2 [z2 [Heq4 Hl4]]].
+      inversion Heq3; subst; clear Heq3.
+      inversion Heq4; subst; clear Heq4.
+      replace i2 with i1 in Hl4; last by lias.
+      rewrite Hl3 in Hl4.
+      by inversion Hl4.
+    }
+    {
+      apply nodup_imap_inj1.
+      move => n1 n2 t1 t2 H2.
+      inversion H2; subst; clear H2.
+      by lias.
+    }
+  }
+  clear Hgunion Hgdisj.
+  iClear "Hgtoken".
+  iInduction ng as [ | g'] "IH" using List.rev_ind => //=.
+  rewrite imap_app.
+  repeat rewrite big_sepL_app.
+  iDestruct "Hgmaps" as "(Hgm1 & Hgm2)".
+  iSplitL "Hgm1"; first by iApply "IH".
+  simpl.
+  by iFrame.
+Qed.
+  
 Lemma instantiation_spec_operational_no_start (s: stuckness) E (hs_mod: N) (hs_imps: list vimp) (v_imps: list module_export) (hs_exps: list vi) (m: module) t_imps t_exps wfs wts wms wgs :
   m.(mod_start) = None ->
   module_typing m t_imps t_exps ->
@@ -1466,7 +1958,7 @@ Lemma instantiation_spec_operational_no_start (s: stuckness) E (hs_mod: N) (hs_i
 Proof.
   
   move => Hmodstart Hmodtype Hmodrestr.
-  iIntros "(Hmod & Himphost & Himpwasm & Hexphost & Hlenexp & %Hebound & %Hdbound)".
+  iIntros "(Hmod & Himphost & Himpwasm & Hexphost & %Hlenexp & %Hebound & %Hdbound)".
   
   repeat rewrite weakestpre.wp_unfold /weakestpre.wp_pre /=.
   
@@ -1559,12 +2051,18 @@ Proof.
 
   remember (fmap (fun m_exp => {| modexp_name := modexp_name m_exp; modexp_desc := export_get_v_ext inst_res (modexp_desc m_exp) |}) m.(mod_exports)) as v_exps.
 
+  remember (init_mems host_function
+    (init_tabs host_function s3 inst_res
+       [seq Z.to_nat (Wasm_int.Int32.intval o) | o <- e_inits] 
+       (mod_elem m)) inst_res
+    [seq Z.to_N (Wasm_int.Int32.intval o) | o <- d_inits] 
+    (mod_data m)) as ws_res.
+  
   (* Prove that the instantiation predicate holds *)
-  assert (exists ws_res, (instantiate ws m (fmap modexp_desc v_imps) ((ws_res, inst_res, v_exps), None))) as Hinst.
+  assert ((instantiate ws m (fmap modexp_desc v_imps) ((ws_res, inst_res, v_exps), None))) as Hinst.
   {
     unfold instantiate, instantiation.instantiate.
     unfold alloc_module => /=.
-    eexists.
     exists t_imps, t_exps, hs, s3, g_inits.
     exists e_inits, d_inits.
     repeat split.
@@ -2058,50 +2556,177 @@ Proof.
       by eauto.
   }
 
-  destruct Hinst as [ws_res Hinst].
-
-  assert (insert_exports vis hs_exps v_exps <> None) as Hinsertvis.
+  assert (length hs_exps = length v_exps) as Hlenexp2.
   {
+    rewrite Hlenexp.
     rewrite Heqv_exps.
-    destruct m.
-    simpl in *.
-    (*
-    elim => /=; destruct mod_exports => //=.
-    move => hs_exp hs_exps IH Hlenexp.
-    inversion Hlenexp; clear Hlenexp.
-    destruct (insert_exports vis hs_exps (list_fmap _ _ _ mod_exports)) eqn:Hinsert => //.
-    exfalso.*)
-    admit.
+    by rewrite map_length.
   }
+
+  (* Assert that the new vis store exists and is what we want *)
+  assert (exists vis', insert_exports vis hs_exps v_exps = Some vis') as Hinsertexp.
+  {
+    destruct (insert_exports vis hs_exps v_exps) as [ovis | ] eqn:Hovis; first by eexists.
+    exfalso.
+    apply insert_exports_none_len in Hovis.
+    by apply Hovis; clear Hovis.
+  }
+
+  assert (length (lookup_export_vi vis <$> hs_imps) = length v_imps) as Hvilen.
+  {
+    by rewrite fmap_length.
+  }
+    
+  assert (those (lookup_export_vi vis <$> hs_imps) = Some v_imps) as Hvilookup.
+  {
+    apply those_projection_backward => //.
+    move => k.
+    rewrite list_lookup_fmap.
+    rewrite fmap_length in Hvilen.
+    destruct (hs_imps !! k) eqn:Hhsimpsk => /=.
+    - destruct (v_imps !! k) eqn:Hvimpsk.
+      + by eapply Himphost in Hhsimpsk => //.
+      + apply lookup_lt_Some in Hhsimpsk.
+        apply lookup_ge_None in Hvimpsk.
+        rewrite Hvilen in Hhsimpsk.
+        by lias.
+    - destruct (v_imps !! k) eqn:Hvimpsk => //.
+      + apply lookup_lt_Some in Hvimpsk.
+        apply lookup_ge_None in Hhsimpsk.
+        rewrite Hvilen in Hhsimpsk.
+        by lias.
+  }
+
+  destruct Hinsertexp as [vis' Hinsertexp].
   
-  iApply fupd_mask_intro; first by set_solver.
+  iApply fupd_mask_intro; first by solve_ndisj.
   
   iIntros "Hmask".
   iSplit.
   
   - destruct s => //.
     iPureIntro.
-    unfold language.reducible.
-
-(*
-    
-    exists [], (([::], [::]): host_expr), (ws_res, insert_exports vis hs_exps v_exps, ms), [].
-    unfold language.prim_step => /=.
+    unfold language.reducible, language.prim_step.
+    exists [::], ([::], map_start None), (ws_res, vis', ms), [::].
     repeat split => //.
-    replace [] with (map_start None) => //.
-    eapply HR_host_step => //.*)
-    admit.
-    (*
-    eapply HR_host_step => //.
-    by rewrite gmap_of_list_lookup in Hmods.
-*)
-        
+    by eapply HR_host_step => //.
   - iIntros ([hes' wes'] [[ws3 vis3] ms3] efs HStep).
     destruct HStep as [HStep [-> ->]].
     inversion HStep; subst; clear HStep.
+    
+    (* Clear out the other two cases first. *)
+
+    3: {
+      (* Wasm reduction is impossible, because we have nothing in the Wasm part. *)
+      by apply empty_no_reduce in H0.
+    }
+    
+    2: {
+      (* oob case is impossible, because we've proven the bound check conditions. *)
+      (* Some preparation work, establishing the relation between wts/wms and the physical store *)
+
+      iDestruct (import_resources_wts_subset with "Hwt Htsize Htlimit Himpwasm") as "%Hwt".
+      specialize (Hwt Hvtlen).
+      
+      iDestruct (import_resources_wms_subset with "Hwm Hmsize Hmlimit Himpwasm") as "%Hwm".
+      specialize (Hwm Hvtlen).
+      
+      exfalso.
+      apply H16. clear H16.
+      (* First clear out some generated variables. *)
+      rewrite Hmod in H4.
+      inversion H4; symmetry in H0; subst; clear H4.
+    
+      rewrite Hvilookup in H13.
+      inversion H13; subst; clear H13.
+
+      split.
+      - by eapply module_elem_bound_check_gmap_extend.
+      - by eapply module_data_bound_check_gmap_extend.
+    }
+
+    (* On to the main branch, the only possible reduction (successful case) *)
+
+    (* Similarly, clear out some generated variables *)
+    rewrite Hmod in H6.
+    inversion H6; symmetry in H0; subst; clear H6.
+    
+    rewrite Hvilookup in H13.
+    inversion H13; subst; clear H13.
+    
     iIntros "!>!>!>".
-    iMod "Hmask".
-    iModIntro.
+
+    (* We need to mass update the state interp. To do that, we first need to retrieve some relations between the resulting variables from inversion and those specified by the precondition -- essentially, instantiation should be a deterministic process. *)
+    (* Now use determinism of instantiation to eliminate a lot of generated variables. *)
+    specialize (instantiate_det _ _ _ _ _ Hinst H15) as Hinsteq.
+
+    destruct ws3.
+    simpl in *.
+    inversion Hinsteq.
+    simpl.
+
+    iDestruct "Himpwasm" as "(Himpdom & Himpwasm)".
+
+  (*  iDestruct (import_resources_wasm_equivalent_aux with "Himpwasm") as "(Himpwf & Himpwt & Himpwm & Himpwg)".*)
+    iFrame "Hmod Himphost".
+    unfold import_resources_wasm_typecheck.
+    unfold instantiation_resources_post.
+    unfold import_resources_host.
+
+    (* We now have to perform the state update step by step... *)
+
+    (* Simplify the state relations first *)
+    destruct ws, s0, s1, s2, s3.
+    simpl in *.
+    
+    (* alloc_funcs *)
+    apply alloc_func_gen_index in Hallocfunc.
+    simpl in Hallocfunc.
+    destruct Hallocfunc as [Hfindex [Hfapp [-> [-> ->]]]].
+    
+    (* alloc_tabs *)
+    apply alloc_tab_gen_index in Halloctab.
+    simpl in Halloctab.
+    destruct Halloctab as [Htindex [Htapp [-> [-> ->]]]].
+    
+    (* alloc_mems *)
+    apply alloc_mem_gen_index in Hallocmem.
+    simpl in Hallocmem.
+    destruct Hallocmem as [Hmindex [Hmapp [-> [-> ->]]]].
+    
+    (* alloc_globs *)
+    apply alloc_glob_gen_index in Hallocglob.
+    simpl in Hallocglob.
+    destruct Hallocglob as [Hgindex [Hgapp [-> [-> ->]]]].
+
+    simpl in *.
+
+    (* Now we perform the state updates *)
+
+    (* alloc_funcs *)
+    iDestruct (alloc_func_state_update with "Hwf") as "Hwf"; first by apply Hfapp.
+
+    iMod "Hwf" as "(Hwf & Hwfmapsto)".
+
+    (* alloc_tabs *)
+    iDestruct (alloc_tab_state_update with "Hwt Htsize Htlimit") as "Hwt"; first by apply Htapp.
+
+    iMod "Hwt" as "(Hwt & Htsize & Htlimit & Htmapsto)".
+    
+    (* alloc_mems *)
+    iDestruct (alloc_mem_state_update with "Hwm Hmsize Hmlimit") as "Hwm"; first by apply Hmapp.
+
+    iMod "Hwm" as "(Hwm & Hmsize & Hmlimit & Hmmapsto)".
+
+    (* alloc_globs *)
+    iDestruct (alloc_glob_state_update with "Hwg") as "Hwg"; first by apply Hgapp.
+
+    iMod "Hwg" as "(Hwg & Hwgmapsto)".
+
+    (* initialisers *)
+
+    (* After the updates to state interp, we just need to provide the remaining bits of equalities in the post-condition. *)
+
 Admitted.
 
 
