theories/iris/stdpp_aux.v
@@ -1,5 +1,6 @@
 From mathcomp Require Import ssreflect eqtype seq ssrbool.
 From stdpp Require Import fin_maps list.
+Require Import list_extra.
 
 Lemma fmap_split: forall {X Y:Type} (f: X -> Y) vs es1 es2,
   fmap f vs = es1 ++ es2 ->
@@ -25,4 +26,28 @@ Proof.
   apply lt_S_n in Hlen.
   f_equal.
   by apply IHl.
+Qed.
+
+Lemma those_projection_backward {T: Type} (l0: list (option T)) (l1: list T):
+  (forall k, match l0 !! k with
+        | Some x => x
+        | None => None
+        end
+        = l1 !! k) ->
+  length l0 = length l1 ->
+  those l0 = Some l1.
+Proof.
+  move: l0 l1.
+  induction l0; destruct l1 => //=; move => H Hlen.
+  specialize (H 0) as H0.
+  simpl in H0.
+  subst.
+  inversion Hlen; clear Hlen.
+  rewrite - those_those0.
+  simpl.
+  unfold option_map.
+  apply IHl0 in H1 => //; first by rewrite those_those0 H1.
+  move => k.
+  specialize (H (S k)).
+  by simpl in H.
 Qed.
